add from_bytes to field

src/Bedrock/Field/Interface/Representation.v
@@ -1,8 +1,10 @@
 Require Import Coq.ZArith.ZArith.
 Require Import Coq.Lists.List.
+Require Import coqutil.Byte.
 Require Import coqutil.Word.Interface.
 Require Import bedrock2.Semantics.
 Require Import Crypto.Arithmetic.Core.
+Require Import Crypto.Arithmetic.ModOps.
 Require Import Crypto.Arithmetic.PrimeFieldTheorems.
 Require Import Crypto.Bedrock.Field.Common.Types.
 Require Import Crypto.Bedrock.Field.Synthesis.Generic.Bignum.
@@ -11,19 +13,34 @@ Require Import Crypto.COperationSpecifications.
 Require Import Crypto.Util.ZRange.
 
 Section Representation.
-  Context {p : Types.parameters} {field_parameters : FieldParameters}.
+  Context {p : Types.parameters} {field_parameters : FieldParameters}
+          {p_ok : Types.ok}.
   Context (n : nat) (weight : nat -> Z)
-          (loose_bounds tight_bounds : list (option zrange)).
+          (loose_bounds tight_bounds : list (option zrange))
+          (relax_bounds :
+             forall X : list Z,
+               list_Z_bounded_by tight_bounds X ->
+               list_Z_bounded_by loose_bounds X).
+  Existing Instance semantics_ok.
 
   Definition eval_words : list word -> F M_pos :=
     fun ws =>
       F.of_Z _ (Positional.eval weight n (map word.unsigned ws)).
 
-  Instance frep : FieldRepresentation :=
+  Definition eval_bytes : list byte -> F M_pos :=
+    fun bs =>
+      F.of_Z _ (Positional.eval
+                           (ModOps.weight 8 1)
+                           (Z.to_nat word_size_in_bytes)
+                           (map byte.unsigned bs)).
+
+  Local Instance frep : FieldRepresentation :=
     { felem := list word;
       feval := eval_words;
+      feval_bytes := eval_bytes;
       felem_size_in_bytes := word_size_in_bytes;
       FElem := Bignum n;
+      FElemBytes := EncodedBignum n;
       bounds := list (option zrange);
       bounded_by :=
         fun bs ws =>
@@ -31,4 +48,22 @@ Section Representation.
       loose_bounds := loose_bounds;
       tight_bounds := tight_bounds;
     }.
+
+  Local Instance frep_ok : FieldRepresentation_ok.
+  Proof.
+    constructor.
+    { cbn [felem_size_in_bytes frep].
+      rewrite word_size_in_bytes_eq.
+
+      (* TODO: should this be upstreamed to bedrock2? *)
+      assert (0 < bytes_per_word width).
+      { cbv [bytes_per_word].
+        pose proof word.width_pos.
+        apply Z.div_str_pos; auto with zarith. }
+
+      cbn [bytes_per]. rewrite Z2Nat.id by auto with zarith.
+      apply Z.mod_same; auto with zarith. }
+    { cbn [bounded_by frep]; intros.
+      apply relax_bounds; auto. }
+  Qed.
 End Representation.
